lib/Lib.Sequence.fsti
@@ -48,6 +48,7 @@ val create:
   -> s:lseq a len{to_seq s == Seq.create len init /\ (forall (i:nat).
     {:pattern (index s i)} i < len ==> index s i == init)}
 
+
 (** Concatenate sequences: use with care, may make implementation hard to verify *)
 val concat:
     #a:Type
@@ -175,18 +176,44 @@ let update_slice
   =
   update_sub #a i start (fin - start) upd
 
+(** Creation of a fixed-length Sequence from an initialization function *)
+val createi: #a:Type 
+  -> len:size_nat 
+  -> init:(i:nat{i < len} -> a)
+  -> s:lseq a len{(forall (i:nat).
+    {:pattern (index s i)} i < len ==> index s i == init i)}
+
+(** Mapi function for fixed-length Sequences *)
+val mapi:#a:Type -> #b:Type -> #len:size_nat
+  -> f:(i:nat{i < len} -> a -> Tot b)
+  -> s1:lseq a len
+  -> s2:lseq b len{(forall (i:nat).
+    {:pattern (index s2 i)} i < len ==> index s2 i == f i s1.[i])}
+
+
 (** Map function for fixed-length Sequences *)
 val map:#a:Type -> #b:Type -> #len:size_nat
-  -> (a -> Tot b)
+  -> f:(a -> Tot b)
+  -> s1:lseq a len
+  -> s2:lseq b len{(forall (i:nat).
+    {:pattern (index s2 i)} i < len ==> index s2 i == f s1.[i])}
+
+(** Map2i function for fixed-length Sequences *)
+val map2i:#a:Type -> #b:Type -> #c:Type -> #len:size_nat
+  -> f:(i:nat{i < len} -> a -> b -> Tot c)
   -> s1:lseq a len
   -> s2:lseq b len
+  -> s3:lseq c len{(forall (i:nat).
+    {:pattern (index s3 i)} i < len ==> index s3 i == f i s1.[i] s2.[i])}
 
 (** Map2 function for fixed-length Sequences *)
 val map2:#a:Type -> #b:Type -> #c:Type -> #len:size_nat
   -> f:(a -> b -> Tot c)
   -> s1:lseq a len
   -> s2:lseq b len
-  -> s3:lseq c len
+  -> s3:lseq c len{(forall (i:nat).
+    {:pattern (index s3 i)} i < len ==> index s3 i == f s1.[i] s2.[i])}
+
 
 (** Forall function for fixed-length Sequences *)
 val for_all:#a:Type -> #len:size_nat -> (a -> Tot bool) -> lseq a len -> bool
